unit tests for QUIC C API

apps/quicMinusNet/quic.c
@@ -67,90 +67,151 @@ int main(int argc, char **argv)
 
   FFI_mitls_init();
 
-  printf("server create\n");
-  if(!FFI_mitls_quic_create(&server, &config, &errmsg))
-  {
-    printf("quic_create server failed: %s\n", errmsg);
-    return -1;
-  }
-
-  config.is_server = 0;
-  config.host_name = "localhost";
-
-  printf("client create\n");
-  if(!FFI_mitls_quic_create(&client, &config, &errmsg))
-  {
-    printf("quic_create client failed: %s\n", errmsg);
-    return -1;
-  }
-
   // server writer buffer (cumulative)
   size_t slen = 0;
   size_t smax = 8*1024; // too much; we use < 1KB
   char *s_buffer = malloc(smax);
-
+  
   // client write buffer (cumulative)
   size_t clen = 0;
   size_t cmax = 8*1024; // too much; we use < 1KB
-  char *c_buffer = malloc(clen); // 
-  int client_complete = 0;
-  int server_complete = 0;
-
-  do{
-    c_buffer += clen; // assuming miTLS never returns a larger clen
-    cmax -= clen;
-    clen = cmax;
-
-    printf("client call clen=%4d slen=%4d\n", clen, slen);
-    rc = FFI_mitls_quic_process(client, s_buffer, &slen, c_buffer, &clen, &errmsg);
-    printf("client done clen=%4d slen=%4d r=%s\n", clen, slen, quic_result_string(rc));
-    dump(c_buffer, clen);
+  char *c_buffer = malloc(clen); //
   
-    client_complete |= rc == TLS_client_complete || rc == TLS_client_complete_with_early_data;
-    if(rc == TLS_error_other || rc == TLS_error_local || rc == TLS_error_alert){
-      printf("Stopping due to error code. Msg: %s\n", errmsg);
-      break;
-    }
+  // buffer for secrets and tickets
+  quic_secret *qs = malloc(sizeof(quic_secret));
+  quic_ticket *qt = malloc(sizeof(quic_ticket));
 
-    s_buffer += slen; // assuming miTLS never returns a larger clen
-    smax -= slen;
-    slen = smax;
+  if (argc == 1) {
+    // GENERIC HANDSHAKE TEST (NO 0RTT) 
     
+      int client_complete = 0;
+      int server_complete = 0;
+
+
+      printf("server create\n");
+      if(!FFI_mitls_quic_create(&server, &config, &errmsg))
+        {
+          printf("quic_create server failed: %s\n", errmsg);
+          return -1;
+        }
+      config.is_server = 0;
+      config.host_name = "localhost";
+      
+      printf("client create\n");
+      if(!FFI_mitls_quic_create(&client, &config, &errmsg))
+        {
+          printf("quic_create client failed: %s\n", errmsg);
+          return -1;
+        }
+      
+      do{
+        c_buffer += clen; // assuming miTLS never returns a larger clen
+        cmax -= clen;
+        clen = cmax;
+        
+        printf("client call clen=%4d slen=%4d\n", clen, slen);
+        rc = FFI_mitls_quic_process(client, s_buffer, &slen, c_buffer, &clen, &errmsg);
+        printf("client done clen=%4d slen=%4d r=%s\n", clen, slen, quic_result_string(rc));
+        dump(c_buffer, clen);
+        
+        client_complete |= rc == TLS_client_complete || rc == TLS_client_complete_with_early_data;
+        if(rc == TLS_error_other || rc == TLS_error_local || rc == TLS_error_alert){
+          printf("Stopping due to error code. Msg: %s\n", errmsg);
+          break;
+        }
+
+        s_buffer += slen; // assuming miTLS never returns a larger clen
+        smax -= slen;
+        slen = smax;
+        
     /* clen -= 12; // simulating fragmentation */
     /* printf("server call clen=%4d slen=%4d\n", clen, slen); */
     /* rs = FFI_mitls_quic_process(server, c_buffer, &clen, s_buffer, &slen, &errmsg); */
     /* printf("server done clen=%4d slen=%4d rc=%d\n", clen, slen, rc); */
     /* clen += 12; */
 
-    printf(" *** START SERVER clen=%4d slen=%4d\n", clen, slen);
-    rs = FFI_mitls_quic_process(server, c_buffer, &clen, s_buffer, &slen, &errmsg);
-    printf(" *** END SERVER clen=%4d slen=%4d r=%s\n", clen, slen, quic_result_string(rs));
-    printf("  === Server output ===\n");
-    dump(s_buffer, slen);
-    printf("  =====================\n");
+        printf("server call clen=%4d slen=%4d\n", clen, slen);
+        rs = FFI_mitls_quic_process(server, c_buffer, &clen, s_buffer, &slen, &errmsg);
+        printf("sender done clen=%4d slen=%4d r=%s\n", clen, slen, quic_result_string(rs));
+        dump(s_buffer, slen);
 
-    server_complete |= rs == TLS_server_complete;
-    if(rs == TLS_error_other || rs == TLS_error_local || rs == TLS_error_alert){
-      printf("Stopping due to error code. Msg: %s\n", errmsg);
-      break;
-    }
+        server_complete |= rs == TLS_server_complete;
+        if(rs == TLS_error_other || rs == TLS_error_local || rs == TLS_error_alert){
+          printf("Stopping due to error code. Msg: %s\n", errmsg);
+          break;
+        }
 
+      }
+      while(!client_complete || !server_complete);
+
+      memset(qs, 0, sizeof(quic_secret));
+      FFI_mitls_quic_get_exporter(server, 0, qs, &errmsg);
+      printf("   === Server exporter secret ===\n");
+      dump(qs->secret, 64);
+      FFI_mitls_quic_get_exporter(client, 0, qs, &errmsg);
+      printf("   === Client exporter secret ===\n");
+      dump(qs->secret, 64);
+      printf("   ==============================\n");
   }
-  while(!client_complete || !server_complete);
 
-  quic_secret *qs = malloc(sizeof(quic_secret));
-  memset(qs, 0, sizeof(quic_secret));
+  if (argc == 2) {
+    // HANDSHAKE WALKTHROUGH; 0RTT then 1RTT
 
-  FFI_mitls_quic_get_exporter(server, 0, qs, &errmsg);
-  printf("   === Server exporter secret ===\n");
-  dump(qs->secret, 64);
-  FFI_mitls_quic_get_exporter(client, 0, qs, &errmsg);
-  printf("   === Client exporter secret ===\n");
-  dump(qs->secret, 64);
-  printf("   ==============================\n");
+    printf("server create\n");
+    if(!FFI_mitls_quic_create(&server, &config, &errmsg))
+      {
+        printf("quic_create server failed: %s\n", errmsg);
+        return -1;
+      }
+    config.is_server = 0;
+    config.host_name = "localhost";
+    
+    printf("client create\n");
+    if(!FFI_mitls_quic_create(&client, &config, &errmsg))
+      {
+        printf("quic_create client failed: %s\n", errmsg);
+        return -1;
+      }
+
+    c_buffer += clen; cmax -= clen; clen = cmax;
+    rc = FFI_mitls_quic_process(client, s_buffer, &slen, c_buffer, &clen, &errmsg);
+    assert(rc == TLS_would_block);
+    printf("client done clen=%4d slen=%4d r=%s\n", clen, slen, quic_result_string(rc));
+    printf("ClientHello[%4d] ---->\n",clen);
+      
+    s_buffer += slen; smax -= slen; slen = smax;
+    rs = FFI_mitls_quic_process(server, c_buffer, &clen, s_buffer, &slen, &errmsg);
+    assert(rs == TLS_server_accept);
+    FFI_mitls_quic_get_exporter(server, 0, qs, &errmsg);
+    printf("server done clen=%4d slen=%4d r=%s\n", clen, slen, quic_result_string(rs));
+    printf("server secret is "); dump(qs->secret, 32);
+    printf("                  <---- ServerHello;(EE; Cert; CertVerify; Finished)[%4d] \n",slen);
+
+    c_buffer += clen; cmax -= clen; clen = cmax;
+    rc = FFI_mitls_quic_process(client, s_buffer, &slen, c_buffer, &clen, &errmsg);
+    assert(rc == TLS_client_complete);
+    FFI_mitls_quic_get_exporter(client, 0, qs, &errmsg);
+    printf("client done clen=%4d slen=%4d r=%s\n", clen, slen, quic_result_string(rc));
+    printf("client secret is "); dump(qs->secret, 32);
+    printf("(Finished) [%4d] ---->\n",clen);
+      
+    s_buffer += slen; smax -= slen; slen = smax;
+    rs = FFI_mitls_quic_process(server, c_buffer, &clen, s_buffer, &slen, &errmsg);
+    assert(rs == TLS_server_complete);
+    printf("server done clen=%4d slen=%4d r=%s\n", clen, slen, quic_result_string(rs));
+    printf("                  <---- {Ticket}[%4d]\n", slen);
+
+    c_buffer += clen; cmax -= clen; clen = cmax;
+    rc = FFI_mitls_quic_process(client, s_buffer, &slen, c_buffer, &clen, &errmsg);
+    assert(rc == TLS_would_block);
+    FFI_mitls_quic_get_ticket(client, qt, &errmsg);
+    printf("client done clen=%4d slen=%4d r=%s\n", clen, slen, quic_result_string(rc));
+    printf("session session is "); dump(qt->ticket, qt->len);
+  }
 
   FFI_mitls_cleanup();
   free(qs);
+  free(qt);
 
   printf("Ok\n");
   return 0;
